PAC/PAC_Checker.thy
@@ -1,0 +1,211 @@
+theory PAC_Checker
+  imports PAC_Polynoms_Operations
+    PAC_Checker_Specification
+    PAC_Map_Rel
+begin
+
+
+
+fun pac_step_rel_raw :: \<open>(nat \<times> nat) set \<Rightarrow> ('a \<times> 'b) set \<Rightarrow> 'a pac_step \<Rightarrow> 'b pac_step \<Rightarrow> bool\<close> where
+\<open>pac_step_rel_raw R1 R2 (AddD p1 p2 i r) (AddD p1' p2' i' r') \<longleftrightarrow>
+   (p1, p1') \<in> R1 \<and> (p2, p2') \<in> R1 \<and> (i, i') \<in> R1 \<and>
+   (r, r') \<in> R2\<close> |
+\<open>pac_step_rel_raw R1 R2 (Add p1 p2 i r) (Add p1' p2' i' r') \<longleftrightarrow>
+   (p1, p1') \<in> R1 \<and> (p2, p2') \<in> R1 \<and> (i, i') \<in> R1 \<and>
+   (r, r') \<in> R2\<close> |
+\<open>pac_step_rel_raw R1 R2 (MultD p1 p2 i r) (MultD p1' p2' i' r') \<longleftrightarrow>
+   (p1, p1') \<in> R1 \<and> (p2, p2') \<in> R2 \<and> (i, i') \<in> R1 \<and>
+   (r, r') \<in> R2\<close> |
+\<open>pac_step_rel_raw R1 R2 (Mult p1 p2 i r) (Mult p1' p2' i' r') \<longleftrightarrow>
+   (p1, p1') \<in> R1 \<and> (p2, p2') \<in> R2 \<and> (i, i') \<in> R1 \<and>
+   (r, r') \<in> R2\<close> |
+\<open>pac_step_rel_raw R1 R2 _ _ \<longleftrightarrow> False\<close>
+
+abbreviation pac_step_rel where
+  \<open>pac_step_rel \<equiv> \<langle>Id, unsorted_poly_rel\<rangle> pac_step_rel_raw\<close>
+
+
+definition check_addition_l :: \<open>_ \<Rightarrow> nat \<Rightarrow> nat \<Rightarrow> nat \<Rightarrow> llist_polynom \<Rightarrow> bool nres\<close> where
+\<open>check_addition_l A p q i r = do {
+   if p \<notin># dom_m A \<or> q \<notin># dom_m A \<or> i \<in># dom_m A
+   then RETURN False
+   else do {
+     ASSERT (p \<in># dom_m A);
+     let p = the (fmlookup A p);
+     ASSERT (q \<in># dom_m A);
+     let q = the (fmlookup A q);
+     pq \<leftarrow> add_poly_l (p, q);
+     weak_equality_p pq r
+   }
+}\<close>
+
+definition check_mult_l :: \<open>_ \<Rightarrow> nat \<Rightarrow>llist_polynom \<Rightarrow>  nat \<Rightarrow> llist_polynom \<Rightarrow> bool nres\<close> where
+\<open>check_mult_l A p q i r = do {
+    if p \<notin># dom_m A \<or> i \<in># dom_m A
+    then RETURN False
+    else do {
+       ASSERT (p \<in># dom_m A);
+       let p = the (fmlookup A p);
+       pq \<leftarrow> mult_poly_full p q;
+       weak_equality_p pq r
+     }
+  }\<close>
+
+(* Copy of WB_More_Refinement *)
+lemma RES_RES_RETURN_RES: \<open>RES A \<bind> (\<lambda>T. RES (f T)) = RES (\<Union>(f ` A))\<close>
+  by (auto simp:  pw_eq_iff refine_pw_simps)
+
+
+lemma check_add_alt_def:
+  \<open>check_add A p q i r =
+    do {
+     if p \<notin># dom_m A \<or> q \<notin># dom_m A \<or> i \<in># dom_m A
+     then RETURN False
+     else do {
+       ASSERT (p \<in># dom_m A);
+       let p = the (fmlookup A p);
+       ASSERT (q \<in># dom_m A);
+       let q = the (fmlookup A q);
+       pq \<leftarrow> add_poly_spec p q;
+       weak_equality pq r
+     }
+  }\<close>
+  by (auto simp: check_add_def weak_equality_def
+      add_poly_spec_def RES_RES_RETURN_RES
+    intro!:  ideal.span_zero
+      exI[of _ \<open>the (fmlookup A p) + the (fmlookup A q)\<close>])
+
+
+
+lemma check_mult_alt_def:
+  \<open>check_mult A p q i r =
+    do {
+     if p \<notin># dom_m A \<or> i \<in># dom_m A
+     then RETURN False
+     else do {
+       ASSERT (p \<in># dom_m A);
+       let p = the (fmlookup A p);
+       pq \<leftarrow> mult_poly_spec p q;
+       weak_equality pq r
+     }
+  }\<close>
+  by (auto simp: check_mult_def weak_equality_def
+      mult_poly_spec_def RES_RES_RETURN_RES
+    intro!:  ideal.span_zero
+      exI[of _ \<open>the (fmlookup A p) * q\<close>])
+
+
+lemma fmap_rel_nat_rel_dom_m[simp]:
+  \<open>(A, B) \<in> \<langle>nat_rel, R\<rangle>fmap_rel \<Longrightarrow> dom_m A = dom_m B\<close>
+  by (subst distinct_set_mset_eq_iff[symmetric])
+    (auto simp: fmap_rel_alt_def distinct_mset_dom)
+
+lemma fmap_rel_nat_the_fmlookup[simp]:
+  \<open>(A, B) \<in> \<langle>S, R\<rangle>fmap_rel \<Longrightarrow> (p, p') \<in> S \<Longrightarrow> p' \<in># dom_m B \<Longrightarrow>
+   (the (fmlookup A p), the (fmlookup B p')) \<in> R\<close>
+  by (auto simp: fmap_rel_alt_def distinct_mset_dom)
+
+lemma ref_two_step':
+  \<open>A \<le> B \<Longrightarrow>  \<Down> R A \<le> \<Down> R B\<close>
+  using ref_two_step by auto
+
+context poly_embed
+begin
+
+abbreviation polys_rel where
+  \<open>polys_rel \<equiv> \<langle>nat_rel, sorted_poly_rel O mset_poly_rel\<rangle>fmap_rel\<close>
+
+
+lemma fref_to_Down_curry:
+  \<open>(uncurry f, uncurry g) \<in> [P]\<^sub>f A \<rightarrow> \<langle>B\<rangle>nres_rel \<Longrightarrow>
+     (\<And>x x' y y'. P (x', y') \<Longrightarrow> ((x, y), (x', y')) \<in> A \<Longrightarrow> f x y \<le> \<Down> B (g x' y'))\<close>
+  unfolding fref_def uncurry_def nres_rel_def
+  by auto
+
+lemma weak_equality_spec_weak_equality:
+  \<open>(p, p') \<in> mset_poly_rel \<Longrightarrow>
+    (r, r') \<in> mset_poly_rel \<Longrightarrow>
+    weak_equality_spec p r \<le> weak_equality p' r'\<close>
+  unfolding weak_equality_spec_def weak_equality_def
+  by (auto simp: mset_poly_rel_def)
+
+
+lemma weak_equality_p_weak_equality_p'[refine]:
+    \<open>weak_equality_p p q \<le> \<Down> bool_rel (weak_equality p' q')\<close>
+    if \<open>(p, p') \<in> sorted_poly_rel O mset_poly_rel\<close>
+      \<open>(q, q') \<in> sorted_poly_rel O mset_poly_rel\<close>
+    for p p' q q'
+    using that
+  by (auto intro!: weak_equality_p_weak_equality_spec[THEN fref_to_Down_curry, THEN order_trans]
+         ref_two_step'
+         weak_equality_spec_weak_equality
+      simp flip: conc_fun_chain)
+
+
+lemma check_addition_l_check_add:
+  assumes \<open>(A, B) \<in> polys_rel\<close> and \<open>(r, r') \<in> sorted_poly_rel O mset_poly_rel\<close>
+  shows
+    \<open>check_addition_l A p q i r \<le> \<Down>bool_rel (check_add B p q i r')\<close>
+proof -
+  have [refine]:
+    \<open>add_poly_l (p, q) \<le> \<Down> (sorted_poly_rel O mset_poly_rel) (add_poly_spec p' q')\<close>
+    if \<open>(p, p') \<in> sorted_poly_rel O mset_poly_rel\<close>
+      \<open>(q, q') \<in> sorted_poly_rel O mset_poly_rel\<close>
+    for p p' q q'
+    using that
+    by (auto intro!: add_poly_l_add_poly_p'[THEN order_trans] ref_two_step'
+         add_poly_p'_add_poly_spec
+      simp flip: conc_fun_chain)
+
+  show ?thesis
+    using assms
+    unfolding check_addition_l_def check_add_alt_def
+    apply refine_rcg
+    subgoal
+      by auto
+    subgoal
+      by auto
+    subgoal
+      by auto
+    subgoal
+      by auto
+    subgoal
+      by (auto simp: fmap_rel_nat_the_fmlookup)
+    done
+qed
+
+
+
+lemma check_mult_l_check_mult:
+  assumes \<open>(A, B) \<in> polys_rel\<close> and \<open>(r, r') \<in> sorted_poly_rel O mset_poly_rel\<close> and
+    \<open>(q, q') \<in> sorted_poly_rel O mset_poly_rel\<close>
+  shows
+    \<open>check_mult_l A p q i r \<le> \<Down>bool_rel (check_mult B p q' i r')\<close>
+proof -
+  have [refine]:
+    \<open>mult_poly_full p q \<le> \<Down> (sorted_poly_rel O mset_poly_rel) (mult_poly_spec p' q')\<close>
+    if \<open>(p, p') \<in> sorted_poly_rel O mset_poly_rel\<close>
+      \<open>(q, q') \<in> sorted_poly_rel O mset_poly_rel\<close>
+    for p p' q q'
+    using that
+    by (auto intro!: mult_poly_full_mult_poly_p'[THEN order_trans] ref_two_step'
+         mult_poly_p'_mult_poly_spec
+      simp flip: conc_fun_chain)
+
+  show ?thesis
+    using assms
+    unfolding check_mult_l_def check_mult_alt_def
+    apply refine_rcg
+    subgoal
+      by auto
+    subgoal
+      by auto
+    subgoal
+      by auto
+    done
+qed
+
+end
+
+end
+
